let rec rev lst = match lst with
    | [] -> []
    | x::xs -> rev xs @ [x]

  prove: rev (l1 @ l2) = rev l2 @ rev l1

  Base case (prove) : rev ([] @ l2)  = rev l2 @ rev []
    = rev l2
    by properties of lists and @
    = rev l2 @ []
    by properties of list and @

    = rev l2 @ rev []
    by definition of reverse



  Inductive case: rev ((x::xs) @ l2) = rev l2 @ rev (x::xs)
  Inductive Hyp: rev (xs @ l2) = rev l2 @ rev xs

  rev ((x::xs) @ l2)
  = rev (x :: (xs @ l2))
   by properties of lists and @
  = rev(xs @ l2) @ [x]
    by def rev
  = (rev l2 @ rev xs) @ [x]
    by inductive hyp.
  = rev l2 @ (rev xs @[x])
   by associativty of  @
  = rev l2 @ rev (x::xs)
    by def of rev

  = rev l2 @ rev (x::xs) is now Proved
